Set_Graphs/Directed_Graphs/Tree_Filter.thy
@@ -1,0 +1,32 @@
+theory Tree_Filter
+  imports "HOL-Data_Structures.Set2_Join"
+begin
+(*by Thomas*)
+(*Filter as another join-based set operation on binary search trees*)
+context Set2_Join
+begin
+
+fun filter where
+"filter P Leaf = Leaf"|
+"filter P (Node l (a, b) r) = 
+ (let l' = filter P l;
+      r' = filter P r
+  in if P a 
+     then join l' a r'
+     else join2 l' r')"
+
+lemma 
+  assumes "inv T \<and> bst T"
+  shows invar_filter: "inv (filter P T) \<and> bst (filter P T)" (is ?th1)
+  and   set_filter: "set_tree (filter P T) = set_tree T \<inter> Collect P" (is ?th2)
+proof-
+  have "?th1 \<and> ?th2"
+    using assms
+  by(induction P T rule: filter.induct)
+    (force intro!: inv_join inv_join2 bst_join bst_join2 dest!: inv_Node)+
+  thus ?th1 ?th2
+    by auto
+qed
+
+end
+end
